src/PreciseFlow.v
@@ -238,14 +238,26 @@ Proof.
   - apply (binds_inert H0) in Hi. split; left*.
   - specialize (IHPf Hi). destruct IHPf as [HT [Hd | Hd]].
     * destruct_all; inversion H.
-      inversions H1. inversions H. inversions H1.
-    * destruct HT as [HT | HT]; split; inversions Hd; inversions H; inversions H1;
+      inversions H1. inversions H. inversions H1. inversion H1.
+      inversion H1. inversion H1. inversion H1.
+    * destruct HT as [HT | HT]; split; inversions Hd; inversions H; repeat inversions H1;
         try solve [left*; right*; eexists; auto];
-        right*; eexists; auto.
+        try solve [right*; left*; eexists; auto];
+        try solve [right*; right*; eexists; auto];
+        try solve [left*; right*; left*; eexists; auto].
+      -- left. right. right. eexists; auto.
+      -- left. right. right. eexists; auto.
   - split*. destruct (IHPf Hi) as [HT [Hd | Hd]]. destruct_all; try solve [inversion H].
     right. inversions H. eexists. apply* open_record_typ_p.
-    subst. right. inversions H. eexists. apply* open_record_typ_p. inversion H. inversion H1.
-    inversion H. inversion H1. inversion Hd. inversion H.
+    subst. right. inversions H. eexists. apply* open_record_typ_p.
+    subst. right. inversions H. eexists. apply* open_record_typ_p.
+    inversion H. inversion H1.
+    inversion H. inversion H1.
+    inversion H. inversion H1.
+    inversion H. inversion H1.
+    inversion H. inversion H1.
+    inversion H. inversion H1.
+    inversions Hd. inversions H.
   - split*. destruct (IHPf Hi) as [HT [Hd | Hd]]; destruct_all; try solve [inversions H; inversion H1];
     inversions Hd; inversions H0; right*.
   - split*. destruct (IHPf Hi) as [HT [Hd | Hd]]; destruct_all; try solve [inversions H; inversion H1];
@@ -271,7 +283,7 @@ Lemma pf_rcd_T : forall G p T U,
     record_type T.
 Proof.
   introv Hi Pf. apply pf_inert in Pf; inversions Pf; eauto. inversion* H. destruct_all. inversions H.
-  inversion H0.
+  inversion H0. inversions H. inversions H0.
 Qed.
 
 (** If a path's environment type is recursive then its precise type is the same recursive type or
@@ -298,8 +310,15 @@ Qed.
 (** If a path's environment type is a singleton type then its precise type is the same
     singleton type. *)
 Lemma pf_sngl_U: forall G p q U,
-    G ⊢! p : {{ q }} ⪼ U->
+    G ⊢! p : {{ q }} ⪼ U ->
     U = {{ q }}.
+Proof.
+  introv Hp. dependent induction Hp; eauto; try (specialize (IHHp _ eq_refl); inversion IHHp).
+Qed.
+
+Lemma pf_tag_U: forall G p q U,
+    G ⊢! p : typ_tag q ⪼ U ->
+    U = typ_tag q.
 Proof.
   introv Hp. dependent induction Hp; eauto; try (specialize (IHHp _ eq_refl); inversion IHHp).
 Qed.
@@ -315,7 +334,8 @@ Proof.
   inversions HT.
   - inversions H. apply pf_forall_U in Pf. inversion Pf.
     apply (pf_rec_rcd_U Hi) in Pf. destruct Pf. inversion* H. inversion H. inversion H1.
-  - inversions H. apply pf_sngl_U in Pf. inversion Pf.
+  - destruct_all. inversions H. apply pf_sngl_U in Pf. inversion Pf.
+    inversions H. apply pf_tag_U in Pf. inversion Pf.
 Qed.
 
 (** If [p]'s precise type is a singleton type then its environment type is the same singleton type. *)
@@ -327,10 +347,27 @@ Proof.
   introv Hi Hp. dependent induction Hp; eauto.
   destruct U; inversions x. lets H: (pf_bnd_T Hi Hp). subst.
   apply (pf_inert Hi) in Hp. inversion* Hp. inversions H. inversion H1. destruct_all.
-  inversion H. inversion H0.
+  inversion H. inversion H0. inversion H. inversion H0.
   lets His: (pf_inertsngl Hi Hp). destruct_all; progress (repeat inversions H0); inversion H1; inversions H0.
-  inversion H3.
+  inversion H2. inversion H2. inversion H3.
   lets His: (pf_inertsngl Hi Hp). destruct_all; progress (repeat inversions H0); inversion H1; inversions H0.
+  inversion H2. inversion H2.
+Qed.
+
+(** If [p]'s precise type is a singleton type then its environment type is the same singleton type. *)
+Lemma pf_tag_T: forall G p q T,
+    inert G ->
+    G ⊢! p : T ⪼ typ_tag q ->
+    T = typ_tag q.
+Proof.
+  introv Hi Hp. dependent induction Hp; eauto.
+  destruct U; inversions x. lets H: (pf_bnd_T Hi Hp). subst.
+  apply (pf_inert Hi) in Hp. inversion* Hp. inversions H. inversion H1. destruct_all.
+  inversion H. inversion H0. inversion H. inversion H0.
+  lets His: (pf_inertsngl Hi Hp). destruct_all; progress (repeat inversions H0); inversion H1; inversions H0.
+  inversion H2. inversion H2. inversion H3.
+  lets His: (pf_inertsngl Hi Hp). destruct_all; progress (repeat inversions H0); inversion H1; inversions H0.
+  inversion H2. inversion H2.
 Qed.
 
 (** If [p]'s precise type is a record, then its envirionment type is a recursive type. *)
@@ -348,11 +385,15 @@ Proof.
   - destruct U; inversions x. apply (pf_bnd_T Hi) in Pf. destruct_all; subst; eauto.
   - inversions H. apply pf_forall_U in Pf. inversion* Pf. eauto.
   - inversions H. apply pf_forall_U in Pf. destruct_all. inversion Pf. eauto.
-  - inversion H1. inversion H2.
-  - inversion H. inversion H0.
+  - inversion H1. inversion H2. inversion H3. inversion H2. inversion H3.
+  - inversion H. inversion H0. inversion H1. inversion H0. inversion H1.
   - destruct U; inversions x. apply pf_bnd_T in Pf. subst*. auto.
-  - inversions H. apply pf_sngl_U in Pf. inversion Pf.
-  - inversions H. apply pf_sngl_U in Pf. inversion Pf.
+  - destruct_all; inversions H.
+    apply pf_sngl_U in Pf. inversion Pf.
+    apply pf_tag_U in Pf. inversion Pf.
+  - destruct_all.
+    inversions H. apply pf_sngl_U in Pf. inversion Pf.
+    inversions H. apply pf_tag_U in Pf. inversion Pf.
 Qed.
 
 (** The following two lemmas express that if [p]'s precise type is a function type,
@@ -367,7 +408,8 @@ Proof.
   inversions Hiu.
   - inversions H. apply pf_forall_U in Pf. inversion* Pf.
     destruct (pf_rec_rcd_U Hi Pf) as [H1 | H1]; inversions H1. inversion H.
-  - inversions H. apply pf_sngl_U in Pf. inversion Pf.
+  - destruct_all. inversions H. apply pf_sngl_U in Pf. inversion Pf.
+    inversions H. apply pf_tag_U in Pf. inversion Pf.
 Qed.
 
 (** A variable [x]'s environment type is [T] then [G(x)=T]. *)
@@ -389,7 +431,9 @@ Proof.
   lets HT: (pf_inert Hi Pf). inversions HT.
   - inversions H. apply pf_forall_U in Pf. inversion Pf.
     destruct (pf_rec_rcd_U Hi Pf); inversion H0; inversion H. inversion H5. inversion H7.
-  - inversions H. apply pf_sngl_U in Pf. inversion Pf.
+  - destruct_all.
+    inversions H. apply pf_sngl_U in Pf. inversion Pf.
+    inversions H. apply pf_tag_U in Pf. inversion Pf.
 Qed.
 
 (** In an inert context, the precise type of a path cannot be type selection. *)
@@ -403,7 +447,9 @@ Proof.
   - inversions H.
     * apply pf_forall_U in Pf. inversion Pf.
     * destruct (pf_rec_rcd_U Hi Pf); inversion H. inversion H1.
-  - destruct H as [r Heq]. subst. apply pf_sngl_U in Pf. inversion Pf.
+  - destruct_all.
+    destruct H as [r Heq]. subst. apply pf_sngl_U in Pf. inversion Pf.
+    destruct H as [r Heq]. subst. apply pf_tag_U in Pf. inversion Pf.
 Qed.
 
 (** The following two lemmas say that if a path's precise type is [...∧ D ∧...]
