src/PreciseTyping.v
@@ -99,7 +99,7 @@ Lemma pt2_inertsngl : forall G p T,
 Proof.
   introv Hi Pf. induction Pf.
   - apply* pf_inertsngl.
-  - left. right. eexists. eauto.
+  - left. right. left. eexists. eauto.
 Qed.
 
 Lemma pt3_inertsngl : forall G p T,
@@ -175,9 +175,11 @@ Proof.
   introv Hi Hp1 Hp2 His. gen T U. induction Hp2; introv Hp1.
   - lets Heq: (pf_T_unique Hi Hp1 H). subst. destruct His.
     * destruct H0. apply* pf_forall_T. apply* pf_bnd_T.
-    * inversions H0. destruct_all. apply* pf_sngl_T.
+    * destruct_all.
+      inversions H0. destruct_all. apply* pf_sngl_T.
+      inversions H0. destruct_all. apply* pf_tag_T.
   - destruct (pf_path_sel _ _ Hi Hp1) as [V Hp].
-    assert (inert_sngl {{ q }}) as His'. { right. eexists. auto. }
+    assert (inert_sngl {{ q }}) as His'. { right. left. eexists. auto. }
     specialize (IHHp2_1 Hi His' _ _ Hp). inversion IHHp2_1.
 Qed.
 
@@ -187,7 +189,7 @@ Lemma pf_pt2_sngl: forall G p T U q,
     G ⊢!! p: {{ q }}->
     T = {{ q }}.
 Proof.
-  introv Hi Hp1 Hp2. apply* pf_pt2. right. eexists. auto.
+  introv Hi Hp1 Hp2. apply* pf_pt2. right. left. eexists. auto.
 Qed.
 
 Lemma field_elim_q0: forall G p q a T,
@@ -286,7 +288,7 @@ Proof.
     * unfold sel_fields in x. destruct p0, p. inversions x.
       lets Hxbs: (pt2_sngl_trans _ Hp Hq0).
       assert (inert_sngl {{ q }}) as His. {
-        right. eexists. eauto.
+        right. left. eexists. eauto.
       }
       simpl in *.
       lets Hu: (pt2_sngl_unique Hi Hpa1 Hxbs).
@@ -563,16 +565,16 @@ Proof.
   introv Hi Hpq Hp Hr. gen q. induction Hp; introv Hpq.
   - constructor.
     assert (inert_sngl {{ q }}) as His. {
-      right. eexists. eauto.
+      right. left. eexists. eauto.
     }
     lets ->: (pt2_sngl_unique' Hi Hpq H). destruct Hr.
     inversion His. inversion H1. inversion H0. inversion H0. inversion H1.
   - specialize (IHHp Hi Hr).
     assert (inert_sngl {{ q }}) as His1. {
-      right. eexists. eauto.
+      right. left. eexists. eauto.
     }
     assert (inert_sngl {{ q0 }}) as His2. {
-      right. eexists. eauto.
+      right. left. eexists. eauto.
     }
     lets Heq: (pt2_sngl_unique' Hi Hpq H). inversions Heq. eauto.
 Qed.
@@ -601,7 +603,7 @@ Proof.
     destruct (pf_bnd_T2 Hi H0) as [V Heq]. subst.
     apply* pf_dec_typ_unique.
   - clear IHHp3. apply pt2 in Hp1. assert (inert_sngl {{ q }}) as His. {
-      right. eexists. eauto.
+      right. left. eexists. eauto.
     }
     lets Hu: (pt2_sngl_unique' Hi H Hp1). inversion Hu.
 Qed.
@@ -783,12 +785,23 @@ Proof.
     apply inert_prefix in Hi; auto.
 Qed.
 
+Lemma pt2_strengthen_one_helper_tag G y bs T x q :
+  inert (G & x ~ T) ->
+  wf G ->
+  G & x ~ T ⊢!! p_sel (avar_f y) bs : typ_tag q ->
+  x <> y ->
+  G ⊢!! p_sel (avar_f y) bs : typ_tag q.
+Proof.
+  intros Hi Hwf Ht Hn. dependent induction Ht.
+  econstructor. apply* pf_strengthen.
+Qed.
+
 Lemma pt2_strengthen_one_helper G y bs T x q :
   inert (G & x ~ T) ->
   wf G ->
   G & x ~ T ⊢!! p_sel (avar_f y) bs : {{ q }}->
   x <> y ->
-  G ⊢!! p_sel (avar_f y) bs : {{ q }}/\ exists S, G ⊢!! q : S.
+  G ⊢!! p_sel (avar_f y) bs : {{ q }} /\ exists S, G ⊢!! q : S.
 Proof.
   intros Hi Hwf Ht Hn. dependent induction Ht.
   - split. econstructor. apply* pf_strengthen.
@@ -801,12 +814,22 @@ Proof.
       apply inert_ok in Hi. intros ->. apply ok_push_inv in Hi as [_ Hq]. eapply binds_fresh_inv; eauto.
     }
     rewrite proj_rewrite in *.
-    pose proof (pt2_inertsngl Hi Ht2) as [[Hin | [q ->]] | Hr].
+    pose proof (pt2_inertsngl Hi Ht2) as [[Hin | [Hin | Hin]] | Hr].
     + pose proof (pt2_to_pf Ht2 (or_introl Hin)) as [? Hpr]. apply pf_strengthen in Hpr; auto; split*.
-    + specialize (IHHt2 _ _ _ _ _ _ Hi Hwf JMeq_refl eq_refl eq_refl Hn') as [IHqx [W IHq']].
+    + inversions Hin.
+      specialize (IHHt2 _ _ _ _ _ _ Hi Hwf JMeq_refl eq_refl eq_refl Hn') as [IHqx [W IHq']].
       split.
       * rewrite proj_rewrite in *. eauto.
       * simpl. eexists; eauto.
+    + inversions Hin.
+      (* specialize (IHHt2 _ _ _ _ _ _ Hi Hwf JMeq_refl eq_refl eq_refl Hn') as [IHqx [W IHq']]. *)
+      split.
+      * eapply pt2_sngl_trans. apply IHy. eapply pt2_strengthen_one_helper_tag.
+        exact Hi. exact Hwf. exact Ht2. exact Hn'.
+      * simpl.
+        eexists; eauto.
+        eapply pt2_strengthen_one_helper_tag. exact Hi. exact Hwf.
+        exact Ht2. exact Hn'.
     + pose proof (pt2_to_pf Ht2 (or_intror Hr)) as [? Hpr]. apply pf_strengthen in Hpr; auto; split*.
 Qed.
 
@@ -818,9 +841,10 @@ Lemma pt2_strengthen_one G y bs T x U :
   G ⊢!! p_sel (avar_f y) bs : U.
 Proof.
   intros Hi Hwf Ht Hn.
-  pose proof (pt2_inertsngl Hi Ht) as [[Hin | [q ->]] | Hr].
+  pose proof (pt2_inertsngl Hi Ht) as [[Hin | [Hin | Hin]] | Hr].
   - pose proof (pt2_to_pf Ht (or_introl Hin)) as [? Hpr]. apply pf_strengthen in Hpr; eauto.
-  - apply* pt2_strengthen_one_helper.
+  - inversions Hin. apply* pt2_strengthen_one_helper.
+  - inversions Hin. apply* pt2_strengthen_one_helper_tag.
   - pose proof (pt2_to_pf Ht (or_intror Hr)) as [? Hpr]. apply pf_strengthen in Hpr; eauto.
 Qed.
 
